src/program_proof/tulip/program/replica/replica_backup.v
@@ -1,0 +1,74 @@
+From Perennial.program_proof.tulip.program Require Import prelude.
+From Perennial.program_proof.tulip.program.replica Require Import
+  replica_repr replica_intervene.
+
+Section program.
+  Context `{!heapGS Σ, !tulip_ghostG Σ}.
+
+  Theorem wp_Replica__Backup (rp : loc) gid rid γ :
+    is_replica rp gid rid γ -∗
+    {{{ True }}}
+      Replica__Backup #rp
+    {{{ RET #(); True }}}.
+  Proof.
+    iIntros "#Hrp" (Φ) "!> _ HΦ".
+    wp_rec.
+
+    (*@ func (rp *Replica) Backup() {                                           @*)
+    (*@     for {                                                               @*)
+    (*@         rp.mu.Lock()                                                    @*)
+    (*@         // Create a copy to not read @rp.ptgsm to simplify proof.       @*)
+    (*@         ptgsm := make(map[uint64][]uint64)                              @*)
+    (*@         for ts, ptgs := range(rp.ptgsm) {                               @*)
+    (*@             ptgsm[ts] = ptgs                                            @*)
+    (*@         }                                                               @*)
+    (*@         for ts, ptgs := range(ptgsm) {                                  @*)
+    (*@             rp.intervene(ts, ptgs)                                      @*)
+    (*@         }                                                               @*)
+    (*@         rp.mu.Unlock()                                                  @*)
+    (*@         primitive.Sleep(params.NS_BACKUP_INTERVAL)                      @*)
+    (*@     }                                                                   @*)
+    (*@ }                                                                       @*)
+    wp_apply (wp_forBreak (λ _, True)%I); wp_pures; last by iApply "HΦ".
+    clear Φ.
+    iIntros (Φ) "!> _ HΦ".
+    iNamed "Hrp".
+    wp_loadField.
+    wp_apply (wp_Mutex__Lock with "Hlock").
+    iIntros "[Hlocked Hrp]".
+    do 2 iNamed "Hrp".
+    iNamed "Hpgm".
+    wp_apply (wp_NewMap).
+    iIntros (mP) "HmP".
+    wp_loadField.
+    set P := (λ (mx : gmap u64 Slice.t), own_map mP (DfracOwn 1) mx)%I.
+    wp_apply (wp_MapIter_fold _ _ _ P with "HptgsmS [$HmP]").
+    { clear Φ.
+      iIntros (m t p Φ) "!> [HmP [%Hnone %Hsome]] HΦ".
+      wp_apply (wp_MapInsert with "HmP"); first done.
+      iIntros "HmP".
+      by iApply "HΦ".
+    }
+    iIntros "[HptgsmS HmP]".
+    subst P. simpl.
+    iAssert (own_replica rp gid rid γ α)%I with "[-HΦ HmP Hlocked]" as "Hrp".
+    { by iFrame "Hcm Hhistm Hcpm Hpsmrkm Hdurable Hlsna ∗ # %". }
+    set P := (λ (mx : gmap u64 Slice.t), own_replica rp gid rid γ α)%I.
+    wp_apply (wp_MapIter_fold _ _ _ P with "HmP [$Hrp]").
+    { clear Φ.
+      iIntros (m t p Φ) "!> [Hrp [%Hnone %Hsome]] HΦ".
+      wp_pures.
+      wp_apply (wp_Replica__intervene with "Hgidrid Hgaddrm Hproph Hinv Hinvfile Hrp").
+      iIntros "Hrp".
+      by iApply "HΦ".
+    }
+    iIntros "[HmP Hrp]".
+    subst P. simpl.
+    wp_loadField.
+    wp_apply (wp_Mutex__Unlock with "[$Hlock $Hlocked $Hrp]").
+    wp_apply (wp_Sleep).
+    wp_pures.
+    by iApply "HΦ".
+  Qed.
+
+End program.
