src/program_proof/tulip/program/replica/replica_intervene.v
@@ -1,0 +1,365 @@
+From Perennial.program_proof.tulip.invariance Require Import execute advance.
+From Perennial.program_proof.tulip.program Require Import prelude.
+From Perennial.program_proof Require Import std_proof.
+From Perennial.program_proof.tulip.program.replica Require Import
+  replica_repr replica_lowest_rank replica_advance replica_log.
+From Perennial.program_proof.tulip.program.backup Require Import
+  btcoord_repr btcoord_finalize start.
+
+Section program.
+  Context `{!heapGS Σ, !tulip_ghostG Σ}.
+
+  Theorem wp_Replica__intervene
+    (rp : loc) (tsW : u64) (ptgsP : Slice.t) rid gid proph γ α :
+    let ts := uint.nat tsW in
+    is_replica_gid_rid rp gid rid -∗
+    is_replica_gaddrm rp γ -∗
+    is_replica_proph rp proph -∗
+    know_tulip_inv_with_proph γ proph -∗
+    know_replica_file_inv γ gid rid -∗
+    {{{ own_replica rp gid rid γ α }}}
+      Replica__intervene #rp #tsW (to_val ptgsP)
+    {{{ RET #(); own_replica rp gid rid γ α }}}.
+  Proof.
+    iIntros (ts) "#Hgidrid #Hgaddrm #Hproph #Hinv #Hinvfile".
+    iIntros (Φ) "!> Hrp HΦ".
+    wp_rec.
+
+    (*@ func (rp *Replica) intervene(ts uint64, ptgs []uint64) {                @*)
+    (*@     var rank uint64 = 2                                                 @*)
+    (*@                                                                         @*)
+    wp_pures.
+    wp_apply (wp_ref_to); first by auto.
+    iIntros (rankP) "HrankP".
+
+    (*@     rankl, ok := rp.lowestRank(ts)                                      @*)
+    (*@     if ok {                                                             @*)
+    (*@         rank = rankl + 1                                                @*)
+    (*@     }                                                                   @*)
+    (*@                                                                         @*)
+    do 2 iNamed "Hrp".
+    wp_apply (wp_Replica__lowestRank with "Hpsmrkm").
+    iIntros (rankl ok) "[Hpsmrkm %Hrankl]".
+    wp_pures.
+
+    (* FIXME: merge the two branches to reduce repeated proof. *)
+    iNamed "Hgidrid".
+    destruct ok; wp_pures.
+    { wp_apply (wp_SumAssumeNoOverflow).
+      iIntros "%Hnof".
+      wp_store.
+
+      (*@     rp.advance(ts, rank)                                                @*)
+      (*@                                                                         @*)
+      wp_load.
+      wp_apply (wp_Replica__advance with "Hpsmrkm").
+      iIntros "Hpsmrkm".
+      rewrite uint_nat_word_add_S; last first.
+      { clear -Hnof. word. }
+
+      (*@     logAdvance(rp.fname, rp.lsna, ts, rank)                             @*)
+      (*@                                                                         @*)
+      wp_load.
+      iNamed "Hfname". iNamed "Hlsna".
+      do 2 wp_loadField.
+      wp_apply wp_logAdvance.
+      (* Open the crash, replica, and file invariants. *)
+      iMod (own_crash_ex_open with "Hdurable") as "[> Hdurable HdurableC]".
+      { solve_ndisj. }
+      iNamed "Hdurable".
+      iNamed "Hinv".
+      iInv "Hinv" as "> HinvO" "HinvC".
+      iInv "Hinvfile" as "> HinvfileO" "HinvfileC".
+      iNamed "HinvfileO".
+      (* Agree on the fname, and merge the two ilog quarter. *)
+      iDestruct (replica_ilog_fname_agree with "Hfname Hilogfname") as %->.
+      iDestruct (replica_ilog_combine with "Hilog Hilogfileinv") as "[Hilog ->]".
+      iApply ncfupd_mask_intro; first solve_ndisj.
+      iIntros "Hmask".
+      (* Give the file points-to to the logging method. *)
+      iFrame "Hfile %".
+      iIntros (bs' failed) "Hfile".
+      destruct failed.
+      { (* Case: Write failed. Close the invariants without any updates. *)
+        iMod "Hmask" as "_".
+        iDestruct (replica_ilog_split with "Hilog") as "[Hilog Hilogfileinv]".
+        iMod ("HinvfileC" with "[Hfile Hilogfileinv]") as "_".
+        { by iFrame "∗ # %". }
+        iMod ("HinvC" with "HinvO") as "_".
+        set dst := ReplicaDurable clog ilog.
+        iMod ("HdurableC" $! dst with "[$Hclog $Hilog]") as "Hdurable".
+        by iIntros "!> %Hcontra".
+      }
+      (* Case: Write succeeded. Update the logical state and re-establish invariant. *)
+      iDestruct "Hfile" as "[Hfile %Hencilog']".
+      iNamed "HinvO".
+      iDestruct (big_sepS_elem_of_acc with "Hgroups") as "[Hgroup HgroupsC]"; first apply Hgid.
+      iDestruct (big_sepS_elem_of_acc with "Hrgs") as "[Hrg HrgsC]"; first apply Hgid.
+      iDestruct (big_sepS_elem_of_acc with "Hrg") as "[Hrp HrgC]"; first apply Hrid.
+      (* First catching up the consistent log. *)
+      destruct Hcloga as [cmdsa ->].
+      iMod (replica_inv_execute with "Hclogalb Hclog Hilog Hgroup Hrp")
+        as "(Hclog & Hilog & Hgroup & Hrp)".
+      (* Then apply the validate transition. *)
+      (* ∅ is a placeholder for participant groups. *)
+      iMod (replica_inv_advance ts (S (uint.nat rankl)) (gid, rid) with "Hclog Hilog Hrp")
+        as "(Hclog & Hilog & Hrp & H)".
+      { apply Hexec. }
+      { rewrite /advance_requirement Hrankl. clear. word. }
+      iDestruct "H" as "(Htokens & #Hvote & %ra & %pa & #Hpromise & %Hlastacp)".
+      (* Close the file, replica, and crash invariants. *)
+      iDestruct (replica_ilog_split with "Hilog") as "[Hilog Hilogfileinv]".
+      iMod "Hmask" as "_".
+      iMod ("HinvfileC" with "[Hfile Hilogfileinv]") as "_".
+      { iFrame "∗ #".
+        iPureIntro.
+        split.
+        { apply Forall_app_2; first apply Hvilog.
+          rewrite Forall_singleton.
+          simpl.
+          split.
+          { clear -Hlencloga HlsnaW. word. }
+          split; word.
+        }
+        { rewrite Hlencloga -HlsnaW.
+          rewrite uint_nat_word_add_S in Hencilog'; last word.
+          done.
+        }
+      }
+      iDestruct ("HgroupsC" with "Hgroup") as "Hgroups".
+      iDestruct ("HrgC" with "Hrp") as "Hrg".
+      iDestruct ("HrgsC" with "Hrg") as "Hrgs".
+      iMod ("HinvC" with "[$Htxnsys $Hkeys $Hgroups $Hrgs]") as "_".
+      set ilog' := ilog ++ _.
+      set dst := ReplicaDurable (clog ++ cmdsa) ilog'.
+      iMod ("HdurableC" $! dst with "[$Hclog $Hilog]") as "Hdurable".
+      iIntros "!> _".
+
+      (*@     cid := tulip.CoordID{ GroupID: rp.gid, ReplicaID: rp.rid }          @*)
+      (*@     btcoord := backup.Start(ts, rank, cid, ptgs, rp.gaddrm, 0, rp.proph) @*)
+      (*@                                                                         @*)
+      wp_pures.
+      do 2 wp_loadField.
+      wp_pures.
+      iNamed "Hgaddrm". iNamed "Hproph".
+      do 2 wp_loadField.
+      wp_load.
+      wp_apply (wp_Start _ _ (gid, rid) with "[] [] [] HgaddrmP Hgaddrm Hinv Hinvnets [Htokens]").
+      { (* rank > 1 *) admit. }
+      { apply Hdomgaddrm. }
+      { apply Hdomaddrm. }
+      { (* [is_lnrz_tid] *) admit. }
+      { (* [safe_backup_txn] *) admit. }
+      { (* is_txnptgs_in_slice ptgsP *) admit. }
+      { by rewrite uint_nat_word_add_S; last word. }
+      iIntros (tcoord) "Htcoord".
+      wp_pures.
+
+      (*@     go func() {                                                         @*)
+      (*@         btcoord.Finalize()                                              @*)
+      (*@     }()                                                                 @*)
+      (*@ }                                                                       @*)
+      wp_apply (wp_fork with "[Htcoord]").
+      { (* Forked thread. *)
+        iNext.
+        wp_apply (wp_BackupTxnCoordinator__Finalize with "Htcoord").
+        by iIntros "Htcoord".
+      }
+      wp_pures.
+      iAssert ([∗ map] t ↦ ps ∈ init_psm ts psm, fast_proposal_witness γ gid rid t ps)%I
+        as "#Hfpw'".
+      { rewrite /init_psm.
+        destruct (psm !! ts) as [ps |] eqn:Hps; first done.
+        iApply big_sepM_insert_2; last done.
+        rewrite /fast_proposal_witness /=.
+        iNamed "Hpromise".
+        iFrame "Hlb".
+        iPureIntro.
+        rewrite /last_accepted_decision Hps in Hlastacp.
+        by destruct Hlastacp as [-> ->].
+      }
+      iApply "HΦ".
+      iModIntro.
+      iFrame "∗ # %".
+      iPureIntro.
+      split.
+      { rewrite /init_psm.
+        destruct (psm !! uint.nat tsW) as [p' |] eqn:Hpsmts.
+        { apply elem_of_dom_2 in Hpsmts.
+          rewrite dom_insert_L.
+          clear -Hpsmts Hdompsmrkm.
+          set_solver.
+        }
+        { rewrite 2!dom_insert_L.
+          clear -Hdompsmrkm.
+          set_solver.
+        }
+      }
+      split; first done.
+      rewrite merge_clog_ilog_snoc_ilog; last done.
+      split.
+      { rewrite Forall_forall.
+        intros [n c] Hilog. simpl.
+        apply elem_of_app in Hilog as [Hilog | Hnewc].
+        { rewrite Forall_forall in Hvicmds. by specialize (Hvicmds _ Hilog). }
+        rewrite elem_of_list_singleton in Hnewc.
+        by inv Hnewc.
+      }
+      { by rewrite /execute_cmds foldl_snoc execute_cmds_unfold Hexec /=. }
+    }
+    { (*@     rp.advance(ts, rank)                                                @*)
+      (*@                                                                         @*)
+      wp_load.
+      wp_apply (wp_Replica__advance with "Hpsmrkm").
+      iIntros "Hpsmrkm".
+
+      (*@     logAdvance(rp.fname, rp.lsna, ts, rank)                             @*)
+      (*@                                                                         @*)
+      wp_load.
+      iNamed "Hfname". iNamed "Hlsna".
+      do 2 wp_loadField.
+      wp_apply wp_logAdvance.
+      (* Open the crash, replica, and file invariants. *)
+      iMod (own_crash_ex_open with "Hdurable") as "[> Hdurable HdurableC]".
+      { solve_ndisj. }
+      iNamed "Hdurable".
+      iNamed "Hinv".
+      iInv "Hinv" as "> HinvO" "HinvC".
+      iInv "Hinvfile" as "> HinvfileO" "HinvfileC".
+      iNamed "HinvfileO".
+      (* Agree on the fname, and merge the two ilog quarter. *)
+      iDestruct (replica_ilog_fname_agree with "Hfname Hilogfname") as %->.
+      iDestruct (replica_ilog_combine with "Hilog Hilogfileinv") as "[Hilog ->]".
+      iApply ncfupd_mask_intro; first solve_ndisj.
+      iIntros "Hmask".
+      (* Give the file points-to to the logging method. *)
+      iFrame "Hfile %".
+      iIntros (bs' failed) "Hfile".
+      destruct failed.
+      { (* Case: Write failed. Close the invariants without any updates. *)
+        iMod "Hmask" as "_".
+        iDestruct (replica_ilog_split with "Hilog") as "[Hilog Hilogfileinv]".
+        iMod ("HinvfileC" with "[Hfile Hilogfileinv]") as "_".
+        { by iFrame "∗ # %". }
+        iMod ("HinvC" with "HinvO") as "_".
+        set dst := ReplicaDurable clog ilog.
+        iMod ("HdurableC" $! dst with "[$Hclog $Hilog]") as "Hdurable".
+        by iIntros "!> %Hcontra".
+      }
+      (* Case: Write succeeded. Update the logical state and re-establish invariant. *)
+      iDestruct "Hfile" as "[Hfile %Hencilog']".
+      iNamed "HinvO".
+      iDestruct (big_sepS_elem_of_acc with "Hgroups") as "[Hgroup HgroupsC]"; first apply Hgid.
+      iDestruct (big_sepS_elem_of_acc with "Hrgs") as "[Hrg HrgsC]"; first apply Hgid.
+      iDestruct (big_sepS_elem_of_acc with "Hrg") as "[Hrp HrgC]"; first apply Hrid.
+      (* First catching up the consistent log. *)
+      destruct Hcloga as [cmdsa ->].
+      iMod (replica_inv_execute with "Hclogalb Hclog Hilog Hgroup Hrp")
+        as "(Hclog & Hilog & Hgroup & Hrp)".
+      (* Then apply the validate transition. *)
+      (* ∅ is a placeholder for participant groups. *)
+      iMod (replica_inv_advance ts 2%nat (gid, rid) with "Hclog Hilog Hrp")
+        as "(Hclog & Hilog & Hrp & H)".
+      { apply Hexec. }
+      { rewrite /advance_requirement Hrankl. clear. word. }
+      iDestruct "H" as "(Htokens & #Hvote & %ra & %pa & #Hpromise & %Hlastacp)".
+      (* Close the file, replica, and crash invariants. *)
+      iDestruct (replica_ilog_split with "Hilog") as "[Hilog Hilogfileinv]".
+      iMod "Hmask" as "_".
+      iMod ("HinvfileC" with "[Hfile Hilogfileinv]") as "_".
+      { iFrame "∗ #".
+        iPureIntro.
+        split.
+        { apply Forall_app_2; first apply Hvilog.
+          rewrite Forall_singleton.
+          simpl.
+          split.
+          { clear -Hlencloga HlsnaW. word. }
+          split; word.
+        }
+        { by rewrite Hlencloga -HlsnaW. }
+      }
+      iDestruct ("HgroupsC" with "Hgroup") as "Hgroups".
+      iDestruct ("HrgC" with "Hrp") as "Hrg".
+      iDestruct ("HrgsC" with "Hrg") as "Hrgs".
+      iMod ("HinvC" with "[$Htxnsys $Hkeys $Hgroups $Hrgs]") as "_".
+      set ilog' := ilog ++ _.
+      set dst := ReplicaDurable (clog ++ cmdsa) ilog'.
+      iMod ("HdurableC" $! dst with "[$Hclog $Hilog]") as "Hdurable".
+      iIntros "!> _".
+
+      (*@     cid := tulip.CoordID{ GroupID: rp.gid, ReplicaID: rp.rid }          @*)
+      (*@     btcoord := backup.Start(ts, rank, cid, ptgs, rp.gaddrm, 0, rp.proph) @*)
+      (*@                                                                         @*)
+      wp_pures.
+      do 2 wp_loadField.
+      wp_pures.
+      iNamed "Hgaddrm". iNamed "Hproph".
+      do 2 wp_loadField.
+      wp_load.
+      wp_apply (wp_Start _ _ (gid, rid) with "[] [] [] HgaddrmP Hgaddrm Hinv Hinvnets [Htokens]").
+      { (* rank > 1 *) admit. }
+      { apply Hdomgaddrm. }
+      { apply Hdomaddrm. }
+      { (* [is_lnrz_tid] *) admit. }
+      { (* [safe_backup_txn] *) admit. }
+      { (* is_txnptgs_in_slice ptgsP *) admit. }
+      { simpl. by replace (uint.nat (W64 2)) with 2%nat by word. }
+      iIntros (tcoord) "Htcoord".
+      wp_pures.
+
+      (*@     go func() {                                                         @*)
+      (*@         btcoord.Finalize()                                              @*)
+      (*@     }()                                                                 @*)
+      (*@ }                                                                       @*)
+      wp_apply (wp_fork with "[Htcoord]").
+      { (* Forked thread. *)
+        iNext.
+        wp_apply (wp_BackupTxnCoordinator__Finalize with "Htcoord").
+        by iIntros "Htcoord".
+      }
+      wp_pures.
+      iAssert ([∗ map] t ↦ ps ∈ init_psm ts psm, fast_proposal_witness γ gid rid t ps)%I
+        as "#Hfpw'".
+      { rewrite /init_psm.
+        destruct (psm !! ts) as [ps |] eqn:Hps; first done.
+        iApply big_sepM_insert_2; last done.
+        rewrite /fast_proposal_witness /=.
+        iNamed "Hpromise".
+        iFrame "Hlb".
+        iPureIntro.
+        rewrite /last_accepted_decision Hps in Hlastacp.
+        by destruct Hlastacp as [-> ->].
+      }
+      iApply "HΦ".
+      iModIntro.
+      iFrame "∗ # %".
+      iPureIntro.
+      split.
+      { rewrite /init_psm.
+        destruct (psm !! uint.nat tsW) as [p' |] eqn:Hpsmts.
+        { apply elem_of_dom_2 in Hpsmts.
+          rewrite dom_insert_L.
+          clear -Hpsmts Hdompsmrkm.
+          set_solver.
+        }
+        { rewrite 2!dom_insert_L.
+          clear -Hdompsmrkm.
+          set_solver.
+        }
+      }
+      split; first done.
+      rewrite merge_clog_ilog_snoc_ilog; last done.
+      split.
+      { rewrite Forall_forall.
+        intros [n c] Hilog. simpl.
+        apply elem_of_app in Hilog as [Hilog | Hnewc].
+        { rewrite Forall_forall in Hvicmds. by specialize (Hvicmds _ Hilog). }
+        rewrite elem_of_list_singleton in Hnewc.
+        by inv Hnewc.
+      }
+      { by rewrite /execute_cmds foldl_snoc execute_cmds_unfold Hexec /=. }
+    }
+  Admitted.
+
+End program.
