src/program_proof/tulip/program/replica/start.v
@@ -13,15 +13,18 @@ Section program.
   Context `{!heapGS Σ, !tulip_ghostG Σ, !paxos_ghostG Σ}.
 
   Theorem wp_start
-    (rid : u64) (addr : chan) (fname : byte_string) (proph : proph_id)
+    (gid rid : u64) (addr : chan) (fname : byte_string) (proph : proph_id)
     (addrmpxP : loc) (fnamepx : byte_string)
     (termc : u64) (terml : u64) (lsnc : u64) (logpx : list byte_string) (addrmpx : gmap u64 chan)
-    (clog : dblog) (ilog : list (nat * icommand)) (addrm : gmap u64 chan) gid γ π :
+    (clog : dblog) (ilog : list (nat * icommand)) (addrm : gmap u64 chan)
+    (gaddrmPP : loc) (gaddrmP : gmap u64 loc) (gaddrm : gmap u64 (gmap u64 chan)) γ π :
     let dstpx := PaxosDurable termc terml logpx lsnc in
     let dstrp := ReplicaDurable clog ilog in
     gid ∈ gids_all ->
     rid ∈ rids_all ->
     addrm !! rid = Some addr ->
+    dom gaddrm = gids_all ->
+    map_Forall (λ _ addrm, dom addrm = rids_all) gaddrm ->
     is_node_wal_fname π rid fnamepx -∗
     is_replica_ilog_fname γ gid rid fname -∗
     (* paxos atomic invariants *)
@@ -34,18 +37,23 @@ Section program.
     know_tulip_inv_with_proph γ proph -∗
     know_replica_file_inv γ gid rid -∗
     know_tulip_network_inv γ gid addrm -∗
+    (* backup coordinator *)
+    own_map gaddrmPP DfracDiscarded gaddrmP -∗
+    ([∗ map] addrmP; addrm ∈ gaddrmP; gaddrm, own_map addrmP DfracDiscarded addrm) -∗
+    ([∗ map] gid ↦ addrm ∈ gaddrm, know_tulip_network_inv γ gid addrm) -∗
     {{{ (* durable states passed to paxos *)
         own_map addrmpxP (DfracOwn 1) addrmpx ∗
         own_crash_ex pxcrashNS (own_paxos_durable π rid) dstpx ∗
         own_crash_ex (stagedG0 := tulip_ghostG0.(@tulip_stagedG Σ))
           rpcrashNS (own_replica_durable γ gid rid) dstrp
     }}}
-      start #rid (to_val addr) #(LitString fname) #addrmpxP #(LitString fnamepx) #proph
+      start #gid #rid (to_val addr) #(LitString fname) #addrmpxP #(LitString fnamepx) #gaddrmPP #proph
     {{{ (rp : loc), RET #rp; is_replica rp gid rid γ }}}.
   Proof.
-    iIntros (dstpx dstrp Hgid Hrid Haddr).
+    iIntros (dstpx dstrp Hgid Hrid Hdomgaddrm Hdomaddrm Haddr).
     iIntros "#Hfnamewal #Hfnameilog #Hinvpx #Hinvpxfile #Hinvpxnet".
     iIntros "#Hinvtxnlog #Hinv #Hinvfile #Hinvnet".
+    iIntros "#HgaddrmP #Hgaddrm #Hinvnets".
     iIntros (Φ).
     iIntros "!> (Haddrmpx & Hdurablepx & Hdurable) HΦ".
     wp_rec. wp_pures.
@@ -134,10 +142,13 @@ Section program.
     (* Make read-only persistent resources. *)
     iMod (readonly_alloc_1 with "mu") as "#HmuP".
     iMod (readonly_alloc_1 with "addr") as "#HaddrP".
+    iMod (readonly_alloc_1 with "gid") as "#HgidP".
     iMod (readonly_alloc_1 with "rid") as "#HridP".
     iMod (readonly_alloc_1 with "idx") as "#HidxP".
     iMod (readonly_alloc_1 with "txnlog") as "#HtxnlogP".
     iMod (readonly_alloc_1 with "fname") as "#HfnameP".
+    iMod (readonly_alloc_1 with "gaddrm") as "#HgaddrmPP".
+    iMod (readonly_alloc_1 with "proph") as "#HprophP".
     iAssert (own_replica_cm rp ∅)%I with "[$txntbl $Htxntbl]" as "Hcm"; first done.
     iAssert (own_replica_histm rp (gset_to_gmap [None] keys_all : gmap dbkey dbhist) α)%I
       with "[Hphysm]" as "Hhistm".
@@ -166,6 +177,11 @@ Section program.
       "[$Hcm $Hhistm $Hcpm $Hpgm $Hptsmsptsm $Hpsmrkm]" as "Hrp".
     { iPureIntro. by rewrite merge_clog_ilog_nil. }
     iAssert (is_replica_idx rp γ α)%I with "[$HidxP $Hidx]" as "#Hidxrp".
+    iAssert (is_replica_gid_rid rp gid rid)%I with "[$HgidP $HridP]" as "#Hgidrid".
+    { done. }
+    iAssert (is_replica_gaddrm rp γ)%I as "#Hgaddrmrp".
+    { by iFrame "# %". }
+    iAssert (is_replica_proph rp proph)%I with "[$HprophP]" as "#Hproph".
     iAssert (is_replica_txnlog rp gid γ)%I with "[$HtxnlogP $Htxnlog]" as "Htxnlogrp".
     wp_apply (wp_Replica__resume with
                "[$Hinv] Hinvfile Hfname Hidxrp Htxnlogrp [$Hrp $Hlsna $Hdurable]").
@@ -225,6 +241,10 @@ Section program.
     (*@                                                                         @*)
     wp_apply wp_fork.
     { by wp_apply (wp_Replica__Applier with "Hrptxnlog"). }
+    wp_pures.
+
+    wp_apply wp_fork.
+    { by wp_apply (wp_Replica__Backup with "Hrptxnlog"). }
     wp_pures.
 
     (*@     return rp                                                           @*)
